secure_api/box/functor_box/Box.Indexing.fst
@@ -24,11 +24,6 @@ module Curve = Spec.Curve25519
 
 type id_log_region = (r:MR.rid{extends r root /\ is_eternal_region r /\ is_below r root})
 
-type honesty =
-  | HONEST
-  | DISHONEST
-  | UNDEFINED
-
 type id_log_value = bool
 let id_log_range = fun id_log_key -> id_log_value
 let id_log_inv (id_log_kt:Type0) (m:MM.map' id_log_kt id_log_range) = True
@@ -39,7 +34,7 @@ abstract noeq type index_module =
   | IM:
     rgn: (id_log_region) ->
     subId: (t:Type0{hasEq t}) -> // express that there is a total order on ids
-    smaller: ((i1:subId) -> (i2:subId) -> (b:bool)) ->
+    smaller: (i1:subId -> i2:subId -> t:Type0{t ==> i1 <> i2}) ->
     total_order_lemma: (i1:subId -> i2:subId -> Lemma
       (requires smaller i1 i2)
       (ensures forall i. i <> i1 /\ i <> i2 /\ smaller i i1 ==> smaller i i2)
@@ -158,19 +153,10 @@ let rec dishonest im i =
   | SUBID i' -> MR.witnessed (MM.contains im.id_log i' false) /\ MR.witnessed (MM.defined im.id_log i')
   | ID (i1,i2) -> dishonest im (SUBID i1) \/ dishonest im (SUBID i2)
 
-//val undefined: (im:index_module) -> (i:meta_id im) -> Tot (t:Type0) (decreases (measure_id im i))
-//let rec undefined im i =
-//  match i with
-//  | SUBID i' -> MR.witnessed (MM.contains im.id_log i' false) /\ MR.witnessed (MM.defined im.id_log i')
-//  | ID (i1,i2) -> undefined im (SUBID i1) \/ undefined im (SUBID i2)
-
-
 type absurd_honest (im:index_module) (i:meta_id im{dishonest im i}) = honest im i
 type absurd_dishonest (im:index_module) (i:meta_id im{honest im i}) = dishonest im i
-//type absurd_undefined (im:index_module) (i:meta_id im{(honest im i \/ dishonest im i)}) = undefined im i
 assume val lemma_honest_and_others_tot: im:index_module -> i:meta_id im{dishonest im i} -> absurd_honest im i -> Lemma (False)
 assume val lemma_dishonest_and_others_tot: im:index_module -> i:meta_id im{honest im i} -> absurd_dishonest im i -> Lemma (False)
-//assume val lemma_undefined_and_others_tot: im:index_module -> i:meta_id im{registered im i /\ (honest im i \/ dishonest im i)} -> absurd_undefined im i -> Lemma (False)
 
 
 val lemma_dishonest_not_others: (im:index_module) -> (i:meta_id im) -> ST unit
@@ -265,264 +251,67 @@ val lemma_fresh2: im:index_module -> i:id im -> h:mem -> Lemma
 let lemma_fresh2 im i h =
   ()
 
-#set-options "--z3rlimit 2000 --max_ifuel 1 --max_fuel 1"
-val lemma_registered_not_fresh: im:index_module -> i:meta_id im -> ST unit
-  (requires (fun h0 -> registered im i))
-  (ensures (fun h0 _ h1 ->
-    h0==h1
-    /\ ~(fresh im i h0)
-  ))
-let rec lemma_registered_not_fresh im i =
-  match i with
-  | SUBID i' ->
-    MR.testify (MM.defined im.id_log i');
-    (match MM.lookup im.id_log i' with
-    | Some _ -> ())
-  | ID i' ->
-    lemma_registered_not_fresh im (SUBID (fst i'));
-    lemma_registered_not_fresh im (SUBID (snd i'))
-
-#set-options "--z3rlimit 500 --max_ifuel 2 --max_fuel 3"
-val is_registered: im:index_module -> i:meta_id im -> ST bool
-  (requires (fun h0 -> True))
-  (ensures (fun h0 b h1 ->
-    h0 == h1
-    /\ (b ==> registered im i)
-  ))
-let rec is_registered im i =
-  MR.m_recall im.id_log;
-  match i with
-  | SUBID i' ->
-    (match MM.lookup im.id_log i' with
-    | Some _ -> true
-    | None ->
-      false)
-  | ID i' ->
-    let b1 = is_registered im (SUBID (fst i')) in
-    let b2 = is_registered im (SUBID (snd i')) in
-    if b1 then
-      MR.testify (MM.defined im.id_log ((fst i')));
-    if b2 then
-       MR.testify (MM.defined im.id_log ((snd i')));
-    b1 && b2
-
-
-val is_fresh: im:index_module -> i:meta_id im -> ST bool
-  (requires (fun h0 -> True))
-  (ensures (fun h0 b h1 ->
-    h0 == h1
-    /\ (b ==> fresh im i h0)
-    /\ (SUBID? i /\ not b ==> registered im i)
-    /\ (SUBID? i /\ not b ==> ~(fresh im i h0))
-    /\ (ID? i /\ not b ==> ~(fresh im i h1))
-    /\ (SUBID? i /\ b ==>
-      (let SUBID i' = i in
-      MM.fresh im.id_log i' h1))
-    /\ (b ==>
-    ((ID? i ==>
-      (let ID (i1,i2) = i in
-      MM.fresh im.id_log i1 h1
-      /\ MM.fresh im.id_log i2 h1))
-      ))
-  ))
-let rec is_fresh im i =
-  MR.m_recall im.id_log;
-  match i with
-  | SUBID i' ->
-    (match MM.lookup im.id_log i' with
-    | Some _ -> false
-    | None ->
-      true)
-  | ID i' ->
-    let b1 = is_fresh im (SUBID (fst i')) in
-    let b2 = is_fresh im (SUBID (snd i')) in
-    b1 && b2
-
-
-
-private val merge_honesty_states: h1:honesty -> h2:honesty -> honesty
-let merge_honesty_states h1 h2 =
-  match h1,h2 with
-  | HONEST,HONEST -> HONEST
-  | _,DISHONEST -> DISHONEST
-  | DISHONEST,_ -> DISHONEST
-  | _,_ -> UNDEFINED
-
-
-#set-options "--z3rlimit 900 --max_ifuel 2 --max_fuel 1"
-val get_honesty: im:index_module -> i:meta_id im -> ST(h:honesty) (decreases (measure_id im i))
+#set-options "--z3rlimit 900 --max_ifuel 1 --max_fuel 2"
+val get_honesty: im:index_module -> i:meta_id im -> ST(b:bool) (decreases (measure_id im i))
   (requires (fun h0 ->
-    True
+    registered im i
   ))
-  (ensures (fun h0 h h1 ->
+  (ensures (fun h0 b h1 ->
     modifies_none h0 h1
     /\ h0==h1
-    /\ (HONEST? h ==> (honest im i))
-    /\ (DISHONEST? h ==> dishonest im i)
-    ///\ (SUBID? i /\ (let SUBID i' = i in MM.contains im.id_log i' true h0) ==> HONEST? h )
-    ///\ (SUBID? i /\ (let SUBID i' = i in MM.contains im.id_log i' true h0) ==> honest im i )
-    ///\ (ID? i /\ (let ID (i1,i2) = i in MM.contains im.id_log i1 true h0 /\ MM.contains im.id_log i2 true h0) ==> HONEST? h )
+    /\ (b <==> (honest im i))
+    /\ (~b <==> dishonest im i)
   ))
 let rec get_honesty im i =
   MR.m_recall im.id_log;
   match i with
   | SUBID i' ->
-    if is_registered im (SUBID i') then
-      MR.testify (MM.defined im.id_log i');
-    (match MM.lookup im.id_log i' with
-    | Some b ->
-      lemma_honest_or_dishonest im (SUBID i');
-      (match b with
-      | true ->
-        lemma_honest_not_others im (SUBID i');
-        MR.testify(MM.contains im.id_log i' true);
-        HONEST
-      | false ->
-        lemma_dishonest_not_others im (SUBID i');
-        MR.testify(MM.contains im.id_log i' false);
-        DISHONEST)
-    | None ->
-      let h=get() in
-      assert(MM.fresh im.id_log i' h);
-      UNDEFINED)
-  | ID i' ->
-    let h1 = get_honesty im (SUBID (fst i')) in
-    let h2 = get_honesty im (SUBID (snd i')) in
-    match merge_honesty_states h1 h2 with
-    | HONEST ->
-      lemma_honest_not_others im (ID i');
-      HONEST
-    | DISHONEST ->
-      lemma_dishonest_not_others im (ID i');
-      DISHONEST
-    | UNDEFINED ->
-      UNDEFINED
-
-
-#set-options "--z3rlimit 900 --max_ifuel 1 --max_fuel 2"
-val get_reg_honesty: im:index_module -> i:meta_id im -> ST(h:honesty) (decreases (measure_id im i))
-  (requires (fun h0 ->
-    registered im i
-  ))
-  (ensures (fun h0 h h1 ->
-    modifies_none h0 h1
-    /\ h0==h1
-    /\ (HONEST? h <==> (honest im i))
-    /\ (DISHONEST? h <==> dishonest im i)
-    /\ (HONEST? h \/ DISHONEST? h)
-  ))
-let rec get_reg_honesty im i =
-  MR.m_recall im.id_log;
-  match i with
-  | SUBID i' ->
     MR.testify (MM.defined im.id_log i');
     (match MM.lookup im.id_log i' with
     | Some b ->
       (match b with
       | true ->
         lemma_honest_not_others im (SUBID i');
-        HONEST
+        true
       | false ->
         lemma_dishonest_not_others im (SUBID i');
-        DISHONEST))
+        false))
   | ID i' ->
-    let h1 = get_reg_honesty im (SUBID (fst i')) in
-    let h2 = get_reg_honesty im (SUBID (snd i')) in
-    match merge_honesty_states h1 h2 with
-    | HONEST ->
+    let b1 = get_honesty im (SUBID (fst i')) in
+    let b2 = get_honesty im (SUBID (snd i')) in
+    match b1 && b2 with
+    | true ->
       lemma_honest_not_others im (ID i');
-      HONEST
-    | DISHONEST ->
+      true
+    | false ->
       lemma_dishonest_not_others im (ID i');
-      DISHONEST
+      false
 
 
-// Maybe unify make_honest/dishonest to parameterized "set_honesty"
-private val make_rec_honest: im:index_module -> i:im.subId -> ST unit
-  (requires (fun h0 -> True))
-  (ensures (fun h0 _ h1 ->
-    (fresh im (SUBID i) h0 ==>
-              (MR.m_sel h1 im.id_log == MM.upd (MR.m_sel h0 im.id_log) i true
-              /\ modifies_just (Set.singleton im.rgn) h0.h h1.h
-              /\ honest im (SUBID i)))
-    /\ (~(fresh im (SUBID i) h0) ==> h0 == h1))
-  )
-let make_rec_honest im i =
-  (match MM.lookup im.id_log i with
-  | Some b -> ()
-  | None ->
-    MM.extend im.id_log i true)
-
-val make_honest: im:index_module -> i:meta_id im -> ST unit
+#set-options "--z3rlimit 2000 --max_ifuel 1 --max_fuel 1"
+val set_honesty: im:index_module -> i:meta_id im -> b:bool -> ST unit
   (requires (fun h0 ->
-    honest im i \/ fresh im i h0
+    fresh im i h0
   ))
   (ensures (fun h0 _ h1 ->
-    honest im i
-    /\ (SUBID? i /\ fresh im i h0 ==>
+    (b ==> honest im i)
+    /\ (~b ==> dishonest im i)
+    /\ (SUBID? i ==>
               (let SUBID i' = i in
-              MR.m_sel h1 im.id_log == MM.upd (MR.m_sel h0 im.id_log) i' true
-              /\ modifies (Set.singleton im.rgn) h0 h1))
-    /\ (SUBID? i /\ ~(fresh im i h0) ==> h0 == h1)
+              MR.m_sel h1 im.id_log == MM.upd (MR.m_sel h0 im.id_log) i' b
+              /\ modifies (Set.singleton im.rgn) h0 h1
+              ))
     /\ (ID? i ==>
            (let ID (i1,i2) = i in
-             ((~(fresh im (SUBID i1) h0) /\ ~(fresh im (SUBID i2) h0)) ==> h0 == h1)
-             /\ (fresh im (SUBID i1) h0 /\ ~(fresh im (SUBID i2) h0) ==> MR.m_sel h1 im.id_log == MM.upd (MR.m_sel h0 im.id_log) i1 true /\ modifies (Set.singleton im.rgn) h0 h1)
-             /\ (fresh im (SUBID i2) h0 /\ ~(fresh im (SUBID i1) h0) ==> MR.m_sel h1 im.id_log == MM.upd (MR.m_sel h0 im.id_log) i2 true /\ modifies (Set.singleton im.rgn) h0 h1)
-             /\ (fresh im (SUBID i1) h0 /\ fresh im (SUBID i2) h0 ==> MR.m_sel h1 im.id_log == MM.upd (MM.upd (MR.m_sel h0 im.id_log) i1 true) i2 true /\ modifies (Set.singleton im.rgn) h0 h1)))
+           MR.m_sel h1 im.id_log == MM.upd (MM.upd (MR.m_sel h0 im.id_log) i1 b) i2 b /\ modifies (Set.singleton im.rgn) h0 h1))
   ))
-let rec make_honest im i =
+let rec set_honesty im i b =
   match i with
     | SUBID i' ->
       (match MM.lookup im.id_log i' with
       | Some b -> ()
       | None ->
-        MM.extend im.id_log i' true)
+        MM.extend im.id_log i' b)
     | ID (i1,i2) ->
-    make_rec_honest im i1;
-    make_rec_honest im i2
-
-private val make_rec_dishonest: im:index_module -> i:im.subId -> ST unit
-  (requires (fun h0 -> True))
-  (ensures (fun h0 _ h1 ->
-    (fresh im (SUBID i) h0 ==>
-              (MR.m_sel h1 im.id_log == MM.upd (MR.m_sel h0 im.id_log) i false
-              /\ modifies_just (Set.singleton im.rgn) h0.h h1.h
-              /\ dishonest im (SUBID i)))
-    /\ (~(fresh im (SUBID i) h0) ==> h0 == h1))
-  )
-let make_rec_dishonest im i =
-  (match MM.lookup im.id_log i with
-  | Some b -> ()
-  | None ->
-    MM.extend im.id_log i false)
-
-val make_dishonest: im:index_module -> i:meta_id im -> ST unit
-  (requires (fun h0 ->
-    dishonest im i \/ fresh im i h0
-  ))
-  (ensures (fun h0 _ h1 ->
-    dishonest im i
-    /\ (SUBID? i /\ fresh im i h0 ==>
-             (let SUBID i' = i in
-             MR.m_sel h1 im.id_log == MM.upd (MR.m_sel h0 im.id_log) i' false
-             /\ modifies (Set.singleton im.rgn) h0 h1))
-  /\ (SUBID? i /\ ~(fresh im i h0) ==> h0 == h1)
-  /\ (ID? i ==>
-         (let ID (i1,i2) = i in
-           ((~(fresh im (SUBID i1) h0) /\ ~(fresh im (SUBID i2) h0)) ==> h0 == h1)
-           /\ (fresh im (SUBID i1) h0 /\ ~(fresh im (SUBID i2) h0) ==> MR.m_sel h1 im.id_log == MM.upd (MR.m_sel h0 im.id_log) i1 false /\ modifies (Set.singleton im.rgn) h0 h1)
-           /\ (fresh im (SUBID i2) h0 /\ ~(fresh im (SUBID i1) h0) ==> MR.m_sel h1 im.id_log == MM.upd (MR.m_sel h0 im.id_log) i2 false /\ modifies (Set.singleton im.rgn) h0 h1)
-           /\ (fresh im (SUBID i1) h0 /\ fresh im (SUBID i2) h0 ==> MR.m_sel h1 im.id_log == MM.upd (MM.upd (MR.m_sel h0 im.id_log) i1 false) i2 false /\ modifies (Set.singleton im.rgn) h0 h1)))
-  ))
-
-let rec make_dishonest im i =
-  match i with
-  | SUBID i' ->
-    (match MM.lookup im.id_log i' with
-    | Some b -> ()
-    | None ->
-      MM.extend im.id_log i' false)
-  | ID (i1,i2) ->
-    make_rec_dishonest im i1;
-    make_rec_dishonest im i2
+    set_honesty im (SUBID i1) b;
+    set_honesty im (SUBID i2) b
